%\documentclass{ximera}
%
%\input{../preamble.tex}
%
%\title[Refresh:]{Summation Notation}
%
%\begin{document}
%\begin{abstract}
%  We review the basic of summation notation.
%\end{abstract}
%\maketitle
%
%\begin{problem}
%  Consider the expression:
%  \[
%  \sum_{i=a}^b c_i
%  \]
%  Here each $c_i$ is a
%\wordChoice{
%    \choice{element}
%    \choice{factor}
%    \choice{index}
%    \choice{letter}
%    \choice{lower limit}
%    \choice[correct]{term}
%    \choice{upper limit}
%  } in the sum, 
%  $i$ is called the \wordChoice{
%    \choice{element}
%    \choice{factor}
%    \choice[correct]{index}
%    \choice{letter}
%    \choice{lower limit}
%    \choice{term}
%    \choice{upper limit}
%  } of summation, $a$ is called the
%  \wordChoice{
%    \choice{element}
%    \choice{factor}
%    \choice{index}
%    \choice{letter}
%    \choice[correct]{lower limit}
%    \choice{term}
%    \choice{upper limit}
%    } of summation,
%  and $b$ is called the
%  \wordChoice{
%    \choice{element}
%    \choice{factor}
%    \choice{index}
%    \choice{letter}
%    \choice{term}
%    \choice[correct]{upper limit}
%  }
%  of summation.
%\end{problem}
%
%\begin{problem}
%  Write the terms of this series:
%  \[
%  \sum_{i=1}^4 \left(7-2i\right)=\answer{5}+\answer{3}+\answer{1}+\answer{-1}
%  \]
%\end{problem}
%
%\begin{problem}
%  Write the terms of this series:
%  \[
%  \sum_{i=1}^4 \left(3i^2-5\right)=\answer{-2}+\answer{7}+\answer{22}+\answer{43}
%  \]
%\end{problem}
%
%\begin{problem}
%  Express the sum
%  \[
%  1^2 + 2^2 + 3^2 + 4^2+\dots+27^2
%  \]
%  in summation notation:
%  \[
%  \sum_{k=1}^{\answer{27}} \answer{k^2}
%  \]
%\end{problem}
%
%\begin{problem}
%  Express the sum
%  \[
%  2 + 2^2 + 2^3 + 2^4+\dots+2^{11}
%  \]
%  in summation notation:
%  \[
%  \sum_{n=1}^{\answer{11}} \answer{2^n}
%  \]
%\end{problem}
%
%
%\begin{problem}
%  Express the sum
%  \[
%  7 + \frac{7^2}{2} + \frac{7^3}3 + \frac{7^4}{4}+\dots+\frac{7^{43}}{43}
%  \]
%  in summation notation:
%  \[
%  \sum_{i=1}^{\answer{43}} \answer{7^i/i}
%  \]
%\end{problem}
%
%\begin{problem}
%  Verify that $\left(\sum_{k = 1}^2 k\right)^2 \ne \sum_{k = 1}^2 k^2$ by computing the value of both sides:
%  \begin{align*}
%      \left(\sum_{k = 1}^2 k\right)^2 &= \answer{9} \\
%      \sum_{k = 1}^2 k^2  &= \answer{5}
%  \end{align*}
%\end{problem}
%
%
%\begin{problem}
%  The following are important algebraic rules of exponents:
%  \begin{enumerate}
%    \item $(ab)^n = a^n b^n$
%    \item $\left( \frac{a}{b} \right)^n = \frac{a^n}{b^n}$
%    \item $(a^n)^m = a^{nm}$
%    \item $a^n a^m = a^{n+m}$
%    \item $\frac{a^n}{a^m} = a^{n - m}$
%    \item $\sqrt[n]{a^m} = a^{m/n}$.
%  \end{enumerate}
%  In the following problems, you will be asked to simplify expressions involving exponents.
%  \begin{multipleChoice}
%    \choice[correct]{I understand}
%    \choice{I do not understand}
%  \end{multipleChoice} 
%\end{problem}
%
%
%
%\begin{problem}
%  One of the most important results that will be introduced is a shortcut for adding the terms in a special type of series, called a \textbf{geometric series}.
%  The formula that will be derived in class states:
%  \[
%    \sum_{k = 0}^n a r^k = \frac{a - ar^{n+1}}{1 - r}
%  \]
%  where $a$ and $r$ are constants.
%  
%  In order to use this formula, it is necessary to be able to write a given expression in this form by using the laws of exponents.
%  
%  For example:
%  \[
%    2^{3k - 1} = 2^{3k} \cdot 2^{-1} = (2^3)^k \cdot \frac{1}{2} = 8^k \cdot \frac{1}{2} = \frac{1}{2} \cdot 8^k
%  \]
%  (Here, $a = 1/2$ and $r = 8$.)
%  
%  The next few questions give practice doing this.
%  
%  \begin{multipleChoice}
%    \choice[correct]{I understand}
%    \choice{I do not understand}
%  \end{multipleChoice}
%\end{problem}
%
%\begin{problem}
%  Write the expression $\frac{4^{k+1}}{3^{2k}}$ in the form $a r^k$ by identifying $a$ and $r$:
%  \begin{align*}
%    a &= \answer{4} \\  
%    r &= \answer{4/9}
%  \end{align*}
%\end{problem}
%
%\begin{problem}
%  Write the expression $\frac{3^{2k + 1}}{2 \cdot 2^k}$ in the form $a r^k$ by identifying $a$ and $r$:
%  \begin{align*}
%    a &= \answer{3/2}\\
%    r &= \answer{9/2}
%  \end{align*}
%\end{problem}
%
%\begin{problem}
%  Select ALL of the statements below that are algebraically correct.
%  \begin{selectAll}
%    \choice[correct]{$\frac{4x^2 - 2x}{3x} = \frac{x(4x-2)}{3x} = \frac{4x - 2}{3}$}
%    \choice{$\frac{2x}{1+x^2} = \frac{2x}{1} + \frac{2x}{x^2} = 2x + \frac{2}{x}$}
%    \choice{$(x - 1)^3 = x^3 - 1$}
%    \choice{$\frac{1}{5x} = 5x^{-1}$}
%    \choice[correct]{$(2x)^3 = 2^3 x^3 = 8x^3$}
%    \choice{$2^{3 + 2k} = 2^3 + 2^{2k}$}
%  \end{selectAll}
%\end{problem}
%
%
%\end{document}
