\documentclass{ximera}

\input{../../preamble.tex}

\author{Jim Talamo}
\license{Creative Commons 3.0 By-bC}


\outcome{}


\begin{document}
\begin{exercise}

Consider the series $\sum_{k=1}^{\infty} \frac{k}{k^3+2k+1}$ and pretend that you know only the definition of convergence for series and none of the convergence tests.  

If we were only concerned about the terms in the \emph{sequence}, $\frac{k}{k^3+2k+1}$, we are trying to sum, we could use growth rates to determine that the dominant term in the numerator is $k$ and that the dominant term in the denominator is

\begin{multipleChoice}
\choice{$1$}
\choice{$2k$}
\choice[correct]{$k^3$}
\end{multipleChoice}

Thus, the rational expression $\frac{k}{k^3+2k+1}$ should behave like $\frac{k}{k^3} = \frac{1}{k^2}$ for large $k$.  

While this lets us determine exactly what the limit of the \emph{sequence} $\frac{k}{k^3+2k+1}$ would be, we have to remember that for the \emph{series} $\sum_{k=1}^{\infty} \frac{k}{k^3+2k+1}$:

\begin{multipleChoice}
\choice[correct]{we are adding infinitely many terms together, so the small discrepancies between $\frac{k}{k^3+2k+1}$ and $\frac{1}{k^2}$ may be important!}
\choice{since the difference between $\frac{k}{k^3+2k+1}$ and $\frac{1}{k^2}$ approaches $0$ as $k$ increases, no further exploration is necessary.}
\end{multipleChoice}

Indeed, note that while it is true that $\frac{k}{k^3+2k+1} $ and $\frac{1}{k^2}$ become arbitrarily close as $n$ grows arbitrarily large, there is a small difference between these for each $n$, and the fact that we are trying to add infinitely many such terms together may be problematic!  Indeed, we think of this as:

\[
\frac{k}{k^3+2k+1} \to \frac{1}{k^2} \quad \textrm{ so } \quad \frac{k}{k^3+2k+1} - \frac{1}{k^2} \to 0  
\]

Since we have an infinite series, the consequence of adding infinitely many such terms tells us that heuristically we are adding infinitely many terms whose difference approaches $0$, or that:

\[
\sum^{\infty} \frac{k}{k^3+2k+1} - \frac{1}{k^2} \to \infty \cdot \answer{0}  
\]

There is no reason \emph{a priori} to conclude that we can gain any insight into a \emph{series} by only studying the sequence whose terms we are adding!  

\begin{exercise}
Indeed, the terms in the sequences $\{a_n\}$ given by $a_n =  \frac{1}{2^n}$ and $\{b_n \}$ given by: $b_n=\frac{1}{2^n} + \frac{1}{n}$ are sequences whose terms become arbitrarily close together as $n$ increases since:

\[
a_n-b_n =  \frac{1}{2^n} - \left(\frac{1}{2^n} + \frac{1}{n}\right) = \answer{-\frac{1}{n}}
\]
and thus the difference tends to $0$.  However:

\begin{multipleChoice}
\choice[correct]{$\sum_{k=1}^n a_k$ is a geometric series with $|r| <1$.  It converges.}
\choice{$\sum_{k=1}^n a_k$ is a geometric series with $|r| >1$.  It diverges.}
\end{multipleChoice}

If $\sum_{k=1}^{\infty} b_k$ converges, then $\sum_{k=1}^{\infty} a_k-b_k$ would converge.  However, $\sum_{k=1}^{\infty} a_k-b_k = \sum_{k=1}^{\infty} -\frac{1}{k}$, which: 

\begin{multipleChoice}
\choice[correct]{diverges; it's a $p$-series with $p =1$.}
\choice{converges; it's a $p$-series with $p=1$.}
\end{multipleChoice}

Hence, $\sum_{k=1}^{\infty} b_k$ diverges.  

What conclusion should we draw?

\begin{multipleChoice}
\choice[correct]{We cannot use the fact that the terms in the \emph{sequences} $\{a_n\}$ and $\{b_n\}$ become arbitrarily close to determine if the \emph{series} $\sum_{k=1}^{\infty} a_k$ and $\sum_{k=1}^{\infty} b_k$ either both converge or both diverge.}
\choice{If two sequences $\{a_n\}$ and $\{b_n\}$ have terms that become arbitrarily close, then $\sum_{k=1}^{\infty} a_k$ and $\sum_{k=1}^{\infty} b_k$ will either both converge or both diverge.}
\end{multipleChoice}

\end{exercise}
We need to establish a sufficient way to compare the behavior of the \emph{series} $\sum_{k=1}^{\infty} \frac{k}{k^3+2k+1}$ and $\sum_{k=1}^{\infty} \frac{1}{k^2}$ by comparing the terms in the  \emph{sequences} $\frac{k}{k^3+2k+1}$ and $\frac{1}{k^2}$.  The comparison tests precisely establish this, and the logic behind the comparison test is explored in the context of a specific example in this exercise.

\begin{exercise}
To begin, recall that the series $\sum_{k=1}^{\infty}  a_k$ converges if:

\begin{multipleChoice}
\choice{$\lim_{n \to \infty} a_n = 0$.}
\choice{$\lim_{n \to \infty} a_n$ exists.}
\choice[correct]{$\lim_{n \to \infty} s_n$ exists, where $s_n = \sum_{k=1}^n a_k$.}
\end{multipleChoice}

There are two strategies for determining if $\lim_{n \to \infty} s_n$ exists:

\begin{itemize}
\item[1.] Find an explicit formula for $s_n$ and use it to compute $\lim_{n \to \infty} s_n$ or determine that it does not exist.
\item[2.] Determine if $\{s_n\}$ is bounded and/or monotonic.   
\end{itemize}

In the present case, it would be very difficult to establish an explicit formula for $s_n$, so we will try to establish existence using the second strategy.  First, recall the previous important ideas regarding the second strategy:

\begin{selectAll}
\choice{If $\{s_n\}$ is monotonic $\lim_{n \to \infty} s_n$ exists.}
\choice{If $\{s_n\}$ is bounded $\lim_{n \to \infty} s_n$ exists.}
\choice[correct]{If $\{s_n\}$ is bounded and monotonic, $\lim_{n \to \infty} s_n$ exists.}
\choice[correct]{If $\{s_n\}$ is increasing, we can show $\lim_{n \to \infty} s_n$ does not exist by showing it is not bounded above.}
\choice{If $\{s_n\}$ is increasing, we can show $\lim_{n \to \infty} s_n$ does not exist by showing it is not bounded below.}
\end{selectAll}

Since we have reasoned before that the \emph{sequences} $\frac{k}{k^3+2k+1}$ and $\frac{1}{k^2}$ should be asymptotically similar (behave the same way as $k$ grows arbitrarily large) it is reasonable to hope that:

\begin{multipleChoice}
\choice[correct]{$\sum_{k=1}^{\infty} \frac{k}{k^3+2k+1}$ converges.}
\choice{$\sum_{k=1}^{\infty} \frac{k}{k^3+2k+1} = \sum_{k=1}^{\infty} \frac{1}{k^2}$.}
\choice{$\sum_{k=1}^{\infty} \frac{k}{k^3+2k+1}$ diverges.}
\end{multipleChoice}

Thus, of the strategies we have for considering the limit of $\{s_n\}$ when we cannot find an explicit formula, we will try to establish:

\begin{selectAll}
\choice[correct]{$\{s_n\}$ is bounded and monotonic, so $\lim_{n \to \infty} s_n$ exists.}
\choice{$\{s_n\}$ is increasing, so we can show $\lim_{n \to \infty} s_n$ does not exist by showing it is not bounded above.}
\end{selectAll}

Since $a_n = \frac{n}{n^3+2n+1} > 0$ for all $n \geq 1$ and $s_n = \sum_{k=1}^n a_k$,  we see that:

\begin{multipleChoice}
\choice[correct]{$\{s_n\}$ is increasing.}
\choice{$\{s_n\}$ is decreasing.}
\choice{$\{s_n\}$ is neither increasing nor decreasing.}
\end{multipleChoice}

Also, note that $n^3 < n^3+2n+1$ for all $n \geq 1$, so:
\begin{multipleChoice}
\choice{$\frac{1}{n^3} < \frac{1}{n^3+2n+1}$}
\choice[correct]{$\frac{1}{n^3} > \frac{1}{n^3+2n+1}$}
\end{multipleChoice}

Thus, multiplying both sides by $n$ gives:

\[
\frac{n}{n^3} > \frac{n}{n^3+2n+1}
\]

Note that $\frac{n}{n^3} = \frac{1}{n^2}$, and since this holds for every value of $n$, it certainly holds for the sums up to this value:

\[
\sum_{k=1}^n \frac{k}{k^3+2k+1} < \sum_{k=1}^n \frac{1}{k^2}
\]

Since $\frac{1}{k^2}$ is positive for every $k$, we know that $\sum_{k=1}^n \frac{1}{k^2} < \sum_{k=1}^{\infty} \frac{1}{k^2}$.  But, $\sum_{k=1}^{\infty} \frac{1}{k^2}$:

\begin{multipleChoice}
\choice[correct]{is a $p$-series with $p>1$, it converges.}
\choice{is a $p$-series with $p>1$, it diverges.}
\choice{is a $p$-series with $p<1$, it converges.}
\choice{is a $p$-series with $p<1$, it diverges.}
\end{multipleChoice}

Thus, since:

\[
s_n = \sum_{k=1}^n \frac{n}{n^3+2n+1} < \sum_{k=1}^{\infty} \frac{1}{k^2}
\]

we see that $\{s_n\}$ is bounded above!

We have thus established that $\{s_n\}$ is bounded and monotonic, so $\lim_{n \to \infty} s_n$ must exist, and hence  $\sum_{k=1}^{\infty} \frac{k}{k^3+2k+1}$ converges.

\begin{exercise}
This logic is precisely the logic that can be used to give a formal proof of the comparison test.  Indeed, if we require all of the $a_k$ terms we are summing to be positive, we can establish $s_n$ is increasing:

\begin{itemize}
\item  If we expect the series to converge, we then are tasked with finding a sequence whose terms are larger that converges (like we did here) to establish an upper bound.  
\item If we expect the series to diverge, we must find a sequence whose terms are smaller that diverges.
\end{itemize}

While the sequence of partial sums does not explicitly appear in the statement of the test, it is nonetheless behind the scenes!  
\end{exercise}
\end{exercise}
\end{exercise}
\end{document}
