\documentclass{ximera}
\input{../../preamble.tex}
\author{Emma Smith Zbarsky}
\license{Creative Commons Attribution 3.0 Unported}
\acknowledgement{https://quadbase.org/questions/q14434v1}
\begin{document}

\begin{exercise}

Find the antiderivative: \[\int (6e^{3r} +12r^3 -5)\; dr\]


\begin{hint}
	This is an antiderivative question. It is looking for the most general
	function $f(r)$ such that $f'(r) = 6e^{3r}+12r^3-5$. To solve this, you
	need to use both the exponential rule and the power rule for
	antiderivatives.
\end{hint}


\begin{hint}
	The exponential rule for antiderivatives says that
	$\int e^u \; du = e^u+C$ and in this case, with $u= 3r$,
	$\frac{du}{dr} = 3$ so $du = 3dr$ and
	\[\int e^{u}\; du = \int e^{3r} 3\; dr\] and thus
	\[\int 6e^{3r}\; dr = 2 \int \left(3e^{3r}\right)\; dr = 2\int e^u\; du = 2e^u +C = 2e^{3r}+C.\]

	The power rule for antiderivatives says that
	\[\int r^m \; dr = \frac{r^{m+1}}{m+1}+C\] whenever $m\neq -1$. In this
	problem, we have one term with $m=3$ and one term with $m=0$, so the
	power rule applies and
	\[\int 12r^3-5\; dr = 12\left(\frac{r^4}{4}\right)-5r+C = 3r^4-5r+C.\]
	All together, \[\int 6e^{3r}+12r^3-5\; dr = 2e^{3r}+3r^4-5r+C.\]
\end{hint}


\begin{multipleChoice}
	\choice{$18e^{3r}+36r^2$}
	\choice{$3e^{3r}+4r^4-5r+C$}
	\choice{$3e^{3r}+4r^4-5r$}
	\choice{$2e^{3r}+3r^4-5r$}
	\choice[correct]{$2e^{3r}+3r^4-5r+C$}
\end{multipleChoice}

\end{exercise}
\end{document}
