\documentclass{ximera}

\input{../../preamble.tex}

\author{Jim Talamo}
\license{Creative Commons 3.0 By-bC}

\outcome{Compute derivatives of Taylor series}


\begin{document}

\begin{exercise}
Given that $\ln(1+x) =\sum_{k=0}^{\infty} \frac{(-1)^{k+1}}{k} x^k$, find the sixth degree Taylor polynomial centered at $x=0$ for the function $g(x) = \int_0^x t^3 \ln(1+2t) \d t$

\[
p_6(x) = \answer{\frac{2}{5}x^5-\frac{1}{3}x^6}
\]

(Use the hint if you're stuck)
\begin{hint}
We begin by exhibiting several nonzero terms in the series centered at $t=0$ for  $\ln(1+t)$:

\[
\ln(1+t) = \answer{0}+\answer{1}t+\answer{-\frac{1}{2}}t^2+\answer{\frac{1}{3}}t^3+\ldots
\]
We may need more terms, but we can exhibit them later if necessary.

\begin{question}
Using the rule of compositions, we can find the series for $\ln(1+2t)$:
\[
\ln(1+2t) = \answer{0}+\answer{2}t+\answer{-2}t^2+\answer{\frac{8}{3}}t^3+\ldots
\]
and the series for $t^3\ln(1+2t)$:
\[
\ln(1+2t) = \answer{2t^4-2t^5+\frac{8}{3}t^6}+\ldots (\textrm{ your answer should include up to the } t^6 \textrm{ term})
\]

\begin{question}
We can now integrate the expression we wrote down above to find:

\begin{align*}
g(x) = \int_0^x t^3 \ln(1+2t) \d t &= \int_0^x \left(2t^4-2t^5+\frac{8}{3}t^6+\ldots\right) \d t \\
&= \eval{\answer{\frac{2}{5}t^5-\frac{1}{3}t^6+\frac{4}{9}t^7} + \ldots }_0^x \\
&= \answer{\frac{2}{5}x^5-\frac{1}{3}x^6+\frac{4}{9}x^7} + \ldots 
\end{align*}

We can now extract the sixth degree Taylor polynomial centered at $x=0$ for $g(x)$:
\[
p_6(x) = \answer{\frac{2}{5}x^5-\frac{1}{3}x^6}
\]

\end{question}
\end{question}
\end{hint}

\end{exercise}
\end{document}
