\documentclass{ximera}

\input{../../preamble.tex}

\author{Jim Talamo}
\license{Creative Commons 3.0 By-bC}


\outcome{}


\begin{document}

\begin{exercise}
Consider the function $f(x) = \sum_{k=0}^{\infty} \frac{k+5}{16^k} (x-3)^{4k}$

\begin{exercise}
Find $f(3)$.

\[
f(3) = \answer{5}
\]
\begin{hint}
Write out a few terms in the sum.  What happens when you evaluate at $x=3$?
\end{hint}
\end{exercise}

%%%%%%%%%%%%%%%%%%
\begin{exercise}
The radius of convergence for the series is $\answer{2}$.

\begin{hint}
You can either use the Ratio Test or the rules for compositions to find this.
\end{hint}

\end{exercise}
%%%%%%%%%%%%%%%%%%
\begin{exercise}
Select all of the following series that converge:

\begin{selectAll}
\choice{The series represented by $f(-2)$}
\choice{The series represented by $f(0)$}
\choice[correct]{The series represented by $f(2)$}
\choice[correct]{The series represented by $f(4)$}
\choice{The series represented by $f(5)$}
\choice{The series represented by $f(7)$}
\end{selectAll}

\begin{hint}
The radius of convergence is $\answer{2}$ and the series is centered at $x=\answer{3}$.  Thus:

The lefthand endpoint for the interval of convergence is $x=\answer{1}$.

The righthand endpoint for the interval of convergence is $x=\answer{5}$.

Note that when $x=5$, we must check the series represented by $f(5)$ separately since this is at the endpoint of the interval of convergence.  Note:

\[
f(5) = \sum_{k=0}^{\infty}  \frac{k+5}{16^k} (5-3)^{4k} = \sum_{k=0}^{\infty}  \frac{k+5}{16^k} (16)^k = \sum_{k=0}^{\infty} (k+5)
\]

Which convergence test can be immediately applied now?
\end{hint}

\end{exercise}
%%%%%%%%%%%%%%%%%%
\begin{exercise}
Find $f^{(52)}(3)$.

\[
f^{(52)}(3) = \answer{\frac{(18)(52)!}{(16)^{13}}}
\]
\end{exercise}
%%%%%%%%%%%%%%%%%%
\begin{exercise}
Find $\lim_{x \to 0} \frac{f(x+3)-5}{2x^4-8x^8}$

\[
\lim_{x \to 0} \frac{f(x+3)-5}{2x^4-8x^8} = \answer{\frac{3}{16}}
\]
\end{exercise}


\end{exercise}
\end{document}
