\documentclass{ximera}

\input{../../preamble.tex}

\author{Jim Talamo and Nicholas Hemleben}
\license{Creative Commons 3.0 By-bC}


\outcome{Compute a Taylor Polynomial}


\begin{document}
\begin{exercise}
Find the indicated Taylor polynomials for the following functions.

For the function $f(x) = \sin (x)$, the third degree Taylor polynomial centered at $x=\frac{\pi}{3}$ is:

\[
p_4(x) =
 \answer{ \frac{\sqrt 3 }{2}}+   \answer{ \frac{1}{2}} \left(x- \frac{\pi}{3}\right) + \answer{- \frac{\sqrt{3}}{4}} \left(x- \frac{\pi}{3}\right)^2 +  \answer{-\frac{1}{12}} \left(x- \frac{\pi}{3}\right)^3  .
 \]

\begin{hint}
If $\sin(x) = a_0 + a_1 \left(x- \frac{\pi}{3}\right) + a_2 \left(x- \frac \pi  3\right)^2 + a_3 \left(x- \frac{\pi}{3}\right)^3 +\ldots $, then $a_n = \frac{f^{(n)} \left(\frac{\pi}{3}\right)}{n!}$.  Make sure you compute the derivatives at $x = \frac{\pi}{3}$.
\end{hint}

\end{exercise}

\begin{exercise}
For the function $f(x) = e^{4x}$, the third degree Taylor polynomial centered at $x=1$ is:

\[ 
p_3(x) =
 \answer{e^4}+ \answer{4e^4} (x-1) + \answer{ 8 e^4} (x- 1)^2 +  \answer{ \frac{32}{3} e^4} (x- 1)^3.
 \]
    
\begin{hint}
If $e^{4x} = a_0 + a_1 (x- 1 ) + a_2 (x- 1 )^2 + a_3 (x- 1)^3 +\ldots $, then $a_n = \frac{f^{(n)} (1)} {n!}$
\end{hint}

\end{exercise}

\begin{exercise}
For the function $f(x) =\sqrt{4+x}$, the third degree Taylor polynomial centered at $x=3$ is:

\[
p_3(x) = \answer{\sqrt{7}+ \frac{1}{2 \sqrt{7}} (x-3) - \frac{1}{56 \sqrt{7}} (x- 3)^2 + \frac{1}{784 \sqrt{7}} (x- 3)^3 }  .
\]
     
\begin{hint}
If $\sqrt{4+x} = a_0 + a_1 (x- 3 ) + a_2 (x- 3 )^2 + a_3 (x- 3)^3 +\ldots $.
Then $a_n = \frac{f^{(n)} (1)} {n!}$
\end{hint}

\begin{hint}
$f(x) =  \sqrt{4+x}= (4+x)^{\frac{1} {2}} $ so $f^{(1)} (x) = \frac{1}{2} (4+x)^{- \frac{1} {2}} $.  Find the other derivatives accordingly.  Note that since the series is centered at $x=3$, the polynomial should be written in powers of $\answer{x-3}$. 
\end{hint}
\end{exercise}

\end{document}
