\documentclass{ximera}

\input{../../preamble.tex}

\author{Jim Talamo}
\license{Creative Commons 3.0 By-bC}


\outcome{Gain practice understanding the Taylor Polynomial coefficient formula}


\begin{document}
\begin{exercise}
The second degree Taylor Polynomial for $f(x)$ centered at $x=0$ is:

\[
p_2(x) =1-3x+4x^2
\]
Suppose that we want to find the second degree Taylor polynomial for $g(x) = xf(x)$ centered at $x=0$.  Follow the steps below:

From the Taylor polynomial for $f(x)$, we find that:

\[
f(0) = \answer{1} \qquad \qquad f'(0) = \answer{-3} \qquad \qquad f''(0) = \answer{2}
\]

\begin{hint}

The coefficients of the Taylor Polynomial and the values of the derivatives of the function are related via the formula:

\[
a_k = \frac{f^{(k)}(c)}{k!}
\]
We have that $c=\answer{0}$, so the desired values can be found by noting that $a_0 = \answer{1}$, $a_1 = \answer{-3}$, and $a_2 = \answer{4}$.   

\end{hint}

\begin{exercise}
Now, the second degree Taylor polynomial for $g(x)$ will be of the form:

\[
P_2(x) = b_0+b_1x+b_2x^2
\]
where $b_k = \frac{g^{(k)}(0)}{k!}$.

So, let's start by computing the various derivatives of $g(x)$ and evaluating them at $x=0$:

\begin{question}
\begin{itemize}
\item  For $g(0)$:

$g(x) = x \cdot f(x)$ so $g(0) = 0 \cdot f(0)$.  thus, $g(0) = \answer{0}$.
\end{itemize}
\end{question}

\begin{question}
\begin{itemize}
\item  For $g'(0)$:

$g'(x) = \answer{1} \cdot f(x)+\answer{x} \cdot f'(x)$ so $g'(0) = f(0)+0 \cdot f'(0)$.  Thus, $g'(0) = \answer{1}$.
\end{itemize}
\end{question}

\begin{question}
\begin{itemize}
\item  For $g''(0)$:

$g''(x) = \answer{2} \cdot f'(x)+\answer{x} \cdot f''(x)$ so $g''(0) = \answer{2}f'(0)+ 0 \cdot f''(0)$.  Thus, $g''(0) = \answer{-6}$.
\end{itemize}
\end{question}

\begin{exercise}
Since $b_k = \frac{g^{(k)}(0)}{k!}$, we find:

\[
b_0 = \answer{0} \qquad \qquad b_1 = \answer{1} \qquad \qquad b_2 = \answer{-3}
\]

Thus, the second degree Taylor polynomial for $g(x)$ is:

\[
P_2(x) = \answer{x-3x^2}
\]
\end{exercise}

\end{exercise}
\end{exercise}
\end{document}
